tls13.v
@@ -2,7 +2,7 @@ From stdpp Require Import base gmap.
 From mathcomp Require Import ssreflect.
 From iris.algebra Require Import agree auth csum gset gmap excl frac.
 From iris.heap_lang Require Import notation proofmode.
-From cryptis Require Import lib term cryptis primitives tactics nown.
+From cryptis Require Import lib term cryptis primitives tactics.
 From cryptis Require Import role session dh.
 
 Set Implicit Arguments.
